src/Interfaces.v
@@ -1,0 +1,327 @@
+(** 
+*)
+
+From Equations Require Import Equations.
+
+From Coq Require Import Arith List Lia Setoid Morphisms.
+Import ListNotations.
+From Clairvoyance Require Import Core Approx ApproxM List Misc LazyQueue.
+
+Set Primitive Projections.
+Set Implicit Arguments.
+Set Contextual Implicit.
+Set Maximal Implicit Insertion.
+
+Definition option_bind {A B} (o : option A) (k : A -> option B) : option B :=
+  match o with
+  | None => None
+  | Some a => k a
+  end.
+
+(* lookups xs [n; m; p] = [xs!!n; xs!!m; xs!!p], or None if out of bounds *)
+Fixpoint lookups {A} (xs : list A) (ns : list nat) : option (list A) :=
+  match ns with
+  | [] => Some []
+  | n :: ns =>
+    option_bind (nth_error xs n) (fun x =>
+    option_map (cons x) (lookups xs ns))
+  end.
+
+Module Pure.
+
+Record Impl (op : Type) : Type :=
+  { value : Type
+  ; raw_eval_op : op -> list value -> list value
+  }.
+
+Definition eval_op {op : Type} {j : Impl op} (o : op) (ns : list nat) (xs : list j.(value))
+  : list j.(value) :=
+  match lookups xs ns with
+  | None => xs  (* noop *)
+  | Some vs => xs ++ j.(raw_eval_op) o vs
+  end.
+
+Fixpoint eval_ops {op : Type} {j : Impl op} (os : list (op * list nat)) (xs : list j.(value))
+  : list j.(value) :=
+  match os with
+  | [] => xs
+  | (o, ns) :: os => eval_ops os (eval_op o ns xs)
+  end.
+
+Module Cost.
+
+Record Impl (op : Type) : Type :=
+  { impl :> Pure.Impl op
+    (* The cost may depend on the input *)
+  ; cost : op -> list impl.(value) -> nat
+  }.
+
+Fixpoint eval {op : Type} {j : Impl op} (os : list (op * list nat)) (xs : list j.(value))
+  : nat :=
+  match os with
+  | [] => 0
+  | (o, ns) :: os => j.(cost) o xs + eval os (eval_op o ns xs)
+  end.
+
+End Cost.
+
+End Pure.
+
+Coercion Pure.Cost.impl : Pure.Cost.Impl >-> Pure.Impl.
+
+Notation costop := Pure.Cost.cost.
+Notation costops := Pure.Cost.eval.
+
+Module Cv.
+
+Record Impl (op : Type) : Type :=
+  { value : Type
+  ; raw_eval_op : op -> list value -> M (list value)
+  }.
+
+Definition eval_op {op : Type} {j : Impl op} (o : op) (ns : list nat) (xs : list j.(value))
+  : M (list j.(value)) :=
+  match lookups xs ns with
+  | None => ret xs  (* noop *)
+  | Some vs => let! vs := j.(raw_eval_op) o vs in ret (xs ++ vs)
+  end.
+
+Fixpoint eval_ops {op : Type} {j : Impl op} (os : list (op * list nat)) (xs : list j.(value))
+  : M (list j.(value)) :=
+  match os with
+  | [] => ret xs
+  | (o, ns) :: os => let! xs := eval_op o ns xs in eval_ops os xs
+  end.
+
+End Cv.
+
+Class ImplApprox (op : Type) (j : Pure.Impl op) (j' : Cv.Impl op) : Type :=
+  { ImplExact :> Exact j.(Pure.value) j'.(Cv.value)
+  ; ImplLessDefined :> LessDefined j'.(Cv.value)
+  ; ImplPreOrder :> PreOrder (less_defined (a := j'.(Cv.value)))
+  ; ImplLub :> Lub j'.(Cv.value)
+  ; ImplLubLaw :> LubLaw j'.(Cv.value)
+  ; raw_eval_mon : forall o,
+      Proper (less_defined ==> less_defined) (j'.(Cv.raw_eval_op) o)
+  }.
+
+Definition sumof {A} (f : A -> nat) : list A -> nat :=
+  fold_right (fun x s => f x + s) 0.
+
+Class ImplCost (op : Type) (j : Pure.Cost.Impl op) (j' : Cv.Impl op) {IA : ImplApprox j j'} : Type :=
+  { debt (* = potential *) : j'.(Cv.value) -> nat
+  ; debts := sumof debt
+  ; debt_lub : forall x y, debt (lub x y) <= debt x + debt y
+  ; raw_eval_cost : forall (o : op) (vs : list j.(Pure.value)),
+      forall output, output `is_approx` j.(Pure.raw_eval_op) o vs ->
+      exists input, input `is_approx` vs /\
+      j'.(Cv.raw_eval_op) o input [[ fun r c =>
+        output `less_defined` r /\
+        debts input + c <= j.(costop) o vs + debts output ]]
+  }.
+
+Arguments ImplCost : clear implicits.
+Arguments ImplCost {op} j j' {IA}.
+
+Lemma less_defined_app {a} {LD : LessDefined a} (xs1 xs2 ys1 ys2 : list a)
+  : xs1 `less_defined` ys1 -> xs2 `less_defined` ys2 ->
+    (xs1 ++ xs2) `less_defined` (ys1 ++ ys2).
+Proof.
+  intros H J; induction H; cbn; [ auto | constructor; auto ].
+Qed.
+
+Lemma less_defined_app_inv {a} {LD : LessDefined a} (xs0 xs1 xs2 : list a)
+  : xs0 `less_defined` (xs1 ++ xs2) ->
+    exists xs01 xs02, xs0 = xs01 ++ xs02 /\
+      xs01 `less_defined` xs1 /\ xs02 `less_defined` xs2.
+Proof.
+  revert xs0. induction xs1 as [ | x xs1 IH]; intros xs0 Hxs0; cbn.
+  - exists [], xs0. split; [reflexivity | split; [ constructor | assumption ] ].
+  - cbn in Hxs0. inversion Hxs0; clear Hxs0; subst.
+    specialize (IH _ H3). destruct IH as (xs01 & xs02 & Hxs0 & Hxs1 & Hxs2).
+    exists (x0 :: xs01), xs02.
+    split; [ cbn; f_equal; auto | ].
+    split; [ constructor; auto | auto ].
+Qed.
+
+Lemma exact_list_app {a aA} {EE : Exact a aA} (xs1 xs2 : list a)
+  : exact (xs1 ++ xs2) = exact xs1 ++ exact xs2.
+Proof. apply map_app. Qed.
+
+Lemma less_defined_lookups {a aA} {EE : Exact a aA} {LD : LessDefined aA}
+    {ns : list nat} {xs ys : list a}
+  : lookups xs ns = Some ys ->
+    forall ysD : list aA, ysD `is_approx` ys ->
+    exists xsD : list aA, xsD `is_approx` xs /\ lookups xsD ns = Some ysD.
+Proof. Admitted.
+
+Lemma nth_lub {a} `{LessDefined a, Lub a} {xs ys : list a} {x : a} {n : nat}
+  : nth_error xs n = Some x ->
+    cobounded xs ys ->
+    exists y, nth_error ys n = Some y /\
+      cobounded x y /\
+      nth_error (lub xs ys) n = Some (lub x y).
+Proof.
+Admitted.
+
+Lemma lookups_lub {a} `{LessDefined a, Lub a} {xs ys xs' : list a} {ns : list nat}
+  : lookups xs ns = Some xs' ->
+    cobounded xs ys ->
+    exists ys',
+      lookups ys ns = Some ys' /\
+      cobounded xs' ys' /\
+      lookups (lub xs ys) ns = Some (lub xs' ys').
+Proof.
+  intros Hns Hcob; revert xs' Hns; induction ns as [ | ? ? IH ]; cbn; intros xs'.
+  - intros Hs; inversion Hs; clear Hs; subst.
+    exists []; split; [ | split ]; do 3 econstructor.
+  - destruct (nth_error _ _) as [ x | ] eqn:Hx; cbn; [ | discriminate ].
+    destruct (lookups xs _) as [ xs'' | ] eqn:Hxs; cbn; [ | discriminate ].
+    intros HH; inversion HH; clear HH; subst.
+    specialize (IH _ eq_refl). destruct IH as (ys' & Hys & Hcobs & Hlub).
+    destruct (nth_lub Hx Hcob) as (y & Hy & Hcoby & Hlub1).
+    exists (y :: ys').
+    rewrite Hy; cbn. rewrite Hys; cbn. split; [ reflexivity | ].
+    rewrite Hlub1; cbn.
+    split; [ apply cobounded_cons; auto | ].
+    rewrite Hlub; cbn. reflexivity.
+Qed.
+
+Section Soundness.
+
+Context {op : Type} (j : Pure.Cost.Impl op) (j' : Cv.Impl op)
+  {IA : ImplApprox j j'} {IC : ImplCost j j'}.
+
+Lemma debts_lub x y : cobounded x y -> debts (lub x y) <= debts x + debts y.
+Proof.
+  induction 1 as [ | ? ? ? ? ? ? IH ] using cobounded_list_ind;
+    cbn; [ reflexivity | ].
+  rewrite IH, debt_lub. clear. generalize (debt x) (debt y). lia.
+Qed.
+
+Lemma debts_app x y : debts (x ++ y) = debts x + debts y.
+Proof.
+  induction x as [ | ? ? IH ]; cbn; [ auto | rewrite IH ].
+  generalize (debt a); lia.
+Qed.
+
+Lemma eval_cost (o : op) (ns : list nat) (vs : list j.(Pure.value)) output
+  : output `is_approx` Pure.eval_op o ns vs ->
+    exists input, input `is_approx` vs /\
+    Cv.eval_op o ns input [[ fun r c =>
+      output `less_defined` r /\
+      debts input + c <= j.(costop) o vs (* TODO: not vs, use ns *) + debts output ]].
+Proof.
+  unfold Cv.eval_op, Pure.eval_op.
+  destruct (lookups vs ns) eqn:E; intros Hout.
+  - rewrite exact_list_app in Hout. apply less_defined_app_inv in Hout.
+    destruct Hout as (out1 & out2 & Hout & Hout1 & Hout2).
+    apply raw_eval_cost in Hout2. destruct Hout2 as (input & Hin & HH).
+    destruct (less_defined_lookups E Hin) as (input' & Hin' & HH').
+    exists (lub input' out1).
+    split; [ apply lub_least_upper_bound; auto | ].
+    destruct (lookups_lub (ys := out1) HH') as (y1 & Hx & Hcob1 & Hy);
+      [ eauto | ].
+    rewrite Hy.
+    mgo. relax; [ | intros ? ? Hr; mgo; rewrite Nat.add_0_r; exact Hr ].
+    eapply optimistic_corelax;
+      [ apply raw_eval_mon, lub_upper_bound_l; eauto | | ].
+    { unfold uc; intros * ? ? []; split.
+      - rewrite H1. apply less_defined_app; [ reflexivity | assumption ].
+      - rewrite <- H2. lia. }
+    relax; [ apply HH | cbn; intros r c [Hr Hc] ].
+    split; [ rewrite Hout; apply less_defined_app; [apply lub_upper_bound_r |]; eauto | ].
+    rewrite debts_lub by eauto. rewrite Hout, debts_app.
+    unfold debts. (* Need to construct input' more carefully *)
+Admitted.
+
+Lemma ImplCostSoundness_aux
+  : forall (os : list (op * list nat)) (vs : list j.(Pure.value)),
+    forall output, output `is_approx` Pure.eval_ops os vs ->
+    exists input, input `is_approx` vs /\
+      Cv.eval_ops os input [[ fun r c =>
+        output `less_defined` r /\ c <= costops (j := j) os vs + debts output ]].
+Proof.
+  induction os as [ | [o ns] os IH ]; intros vs output Hout; cbn.
+  - exists output. split; [apply Hout | ].
+    apply optimistic_ret. split; [ reflexivity | apply Nat.le_0_l ].
+  - cbn in Hout. specialize (IH (Pure.eval_op o ns vs) output Hout).
+    destruct IH as (input & Hin & IH).
+    apply eval_cost in Hin.
+Admitted.
+
+Theorem ImplCostSoundness
+  : forall os : list (op * list nat),
+    forall d, d `is_approx` Pure.eval_ops os [] ->
+      Cv.eval_ops os [] [[ fun r c =>
+        d `less_defined` r /\ c <= costops (j := j) os [] + debts d ]].
+Proof.
+  intros os d Hd. destruct (ImplCostSoundness_aux os [] Hd) as (d0 & Hd0 & HH).
+  inversion Hd0; clear Hd0; subst.
+  exact HH.
+Qed.
+
+End Soundness.
+
+(* Example *)
+Module Queue.
+
+Definition a := nat.
+
+Inductive Op : Type :=
+| Init (x : a)
+| Empty
+| Push
+| Pop
+.
+
+Inductive Value : Type :=
+| Q (q : Queue a)
+| E (x : a)
+.
+
+Definition raw_eval (o : Queue.Op) (vs : list Value) : list Value :=
+  match o, vs with
+  | Empty, _ => [Q empty]
+  | Push, Q q :: E x :: _ => [Q (push q x)]
+  | Pop, Q q :: _ =>
+    match pop q with
+    | None => []
+    | Some (x, q) => [E x; Q q]
+    end
+  | Init x, _ => [E x]
+  | _, _ => []
+  end.
+
+Canonical j : Pure.Impl Queue.Op :=
+  {| Pure.value := Value ; Pure.raw_eval_op := raw_eval |}.
+
+Definition cost (_ : Queue.Op) (_ : list Value) : nat := 7.
+
+Module Cv.
+
+Inductive Value : Type :=
+| Q (q : T (QueueA a))
+| E (x : T a)
+.
+
+Definition raw_eval (o : Queue.Op) (vs : list Value) : M (list Value) :=
+  match o, vs with
+  | Empty, _ => let~ q := emptyA in ret [Q q]
+  | Push, Q q :: E x :: _ => let~ q' := pushA q x in ret [Q q']
+  | Pop, Q q :: _ =>
+    let! pop_q := popA q in
+    match pop_q with
+    | None => ret []
+    | Some (x, q) => ret [E x; Q q]
+    end
+  | Init x, _ => ret [E (Thunk x)]
+  | _, _ => ret []
+  end.
+
+Canonical j : Cv.Impl Queue.Op :=
+  {| Cv.value := Value ; Cv.raw_eval_op := raw_eval |}.
+
+End Cv.
+
+End Queue.
